finish parser for intermediate format

src/InterParse.v
@@ -41,25 +41,29 @@ Module InterParse.
     Inductive Desc' : Set := 
     | D_BOOL
     | D_INT
-    | D_NEST (fields : gmap w8 Desc').
+    | D_NEST (fields : gmap Z Desc').
 
-  (* The "problem" with this definition is that it combines incomplete primitive fields with
-     nested ones, i.e. we can have D_BOOL as a stand-alone descriptor but that can't be serialized
-     without knowing what the field number is.
-   *)
+    (* The "problem" with this definition is that it combines incomplete
+     primitive fields with nested ones, i.e. we can have D_BOOL as a stand-alone
+     descriptor but that can't be serialized without knowing what the field
+     number is. *)
 
-    Inductive Desc : Set := DESC (fs : gmap w8 Field)
+    Inductive Desc : Set := DESC (fs : gmap Z Field)
     with
       Field :=
     | F_MSG (d : Desc)
     | F_BOOL
     | F_INT.
     
-  (* Instead, use a mutually recursive type so that fields and descriptors (fields with an identifier)
-     are distinct.
-   *)
+    Definition Fields (d : Desc) : gmap Z Field :=
+      match d with
+      | DESC fs => fs
+      end.
+    
+    (* Instead, use a mutually recursive type so that fields and descriptors
+     (fields with an identifier) are distinct. *)
 
-    Inductive Value : Set := VALUE (vs : gmap w8 Val)
+    Inductive Value : Set := VALUE (vs : gmap Z Val)
     with
       Val :=
     | V_MSG (v : Value)
@@ -67,47 +71,323 @@ Module InterParse.
     | V_INT (b : Z)
     | V_MISSING.
 
-  (* Define a Value type which matches the structure of the descriptor, with an extra option for
-     missing values, which will also be used as a default value when creating an empty value. *)
+    Definition Vals (v : Value) : gmap Z Val :=
+      match v with
+      | VALUE vs => vs
+      end.
+
+    (* We will also need be able to make an empty value for each descriptor *)
+
+    Fixpoint Init (d : Desc) : Value :=
+      match d with
+      | DESC fs => VALUE $ map_fold (Init__fold) gmap_empty fs
+      end
+    with Init__fold (k : Z) (f : Field) (acc : gmap Z Val) : gmap Z Val :=
+           match f with
+           | F_MSG d => <[ k := V_MSG (Init d) ]> acc
+           | _ => <[ k := V_MISSING ]> acc
+           end.
+
+    (* Fixpoint Eqb (v1 v2 : Value) : bool := *)
+    (*   match v1, v2 with *)
+    (*   | VALUE vs1, VALUE vs2 => andb (map_fold (Eqb__fold vs1) true vs2) *)
+    (*                                 (map_fold (Eqb__fold vs2) true vs1) *)
+    (*   end *)
+    (* with Eqb__fold (vs : gmap Z Val) (k : Z) (v : Val) (acc : bool) : bool := *)
+    (*        if negb acc then *)
+    (*          (* If we already know it isn't a subset, just feed forward *) *)
+    (*          acc *)
+    (*        else *)
+    (*          match vs !! k with *)
+    (*          | Some (V_BOOL b') => match v with *)
+    (*                              | V_BOOL b => bool_eq b' b *)
+    (*                              | _ => false *)
+    (*                              end *)
+    (*          | Some (V_INT z') => match v with *)
+    (*                             | V_INT z => Z.eqb z' z *)
+    (*                             | _ => false *)
+    (*                             end *)
+    (*          | Some V_MISSING => match v with *)
+    (*                             | V_MISSING => true *)
+    (*                             | _ => false *)
+    (*                             end *)
+    (*          | Some (V_MSG v') => match v with *)
+    (*                              | V_MSG v'' => Eqb v' v'' *)
+    (*                              | _ => false *)
+    (*                              end *)
+    (*          | None => false *)
+    (*          end. *)
+    (* FIXME: Error: Cannot guess decreasing argument of fix. *)
+
+    (* Define a Value type which matches the structure of the descriptor, with
+     an extra option for missing values, which will also be used as a default
+     value when creating an empty value. *)
     
-  (* Now in order to use the RecursiveState combinator we need a proposition linking
-     a Value to it's Descriptor. Valid : Desc -> Value -> Prop *)
+    (* Now in order to use the RecursiveState combinator we need a proposition
+     linking a Value to it's Descriptor. Valid : Desc -> Value -> Prop *)
+
+    (* Specifically, this requires that each field in the descriptor exists in
+     the value, has the correct type and isn't missing. Values are allowed to have
+     more fields than the descriptor under this definition. That should be OK, since
+     those unknown fields will be dropped during the parsing process. *)
 
     Fixpoint Valid (d : Desc) (v : Value) : Prop :=
       match d, v with
       | DESC fs, VALUE vs => map_fold (Valid__fold vs) True fs
       end
-    with Valid__fold (vs : gmap w8 Val) (k : w8) (f : Field) (acc : Prop) : Prop :=
+    with Valid__fold (vs : gmap Z Val) (k : Z) (f : Field) (acc : Prop) : Prop :=
            match f with
            | F_BOOL => acc /\ exists b, vs !! k = Some (V_BOOL b)
            | F_INT => acc /\ exists z, vs !! k = Some (V_INT z)
            | F_MSG d => acc /\ exists v, vs !! k = Some (V_MSG v) /\ Valid d v
            end.
+    Opaque Valid.
 
     Definition desc1 := DESC (list_to_map [
-                                  (W8 1, F_BOOL);
-                                  (W8 2, F_INT)
+                                  (1, F_BOOL);
+                                  (2, F_INT)
                           ]).
     Definition val1 := VALUE (list_to_map [
-                                  (W8 1, V_BOOL false);
-                                  (W8 2, V_INT 0)
+                                  (1, V_BOOL false);
+                                  (2, V_INT 0)
                          ]).
+
     Lemma test_valid1 : Valid desc1 val1.
     Proof.
-      simpl.
-      unfold map_fold.
-      unfold gmap_fold. 
-    Abort.
+      vm_compute. rewrite ?Logic.and_assoc.
+      split; first trivial.
+      split; first (exists false; reflexivity).
+      exists 0; reflexivity.
+    Qed.
+
+    Compute Init desc1.
+
+    Definition desc2 := DESC (list_to_map [
+                                  (1, F_MSG desc1);
+                                  (2, F_BOOL)
+                          ]).
+    Definition val2 := VALUE (list_to_map [
+                                (1, V_MSG val1);
+                                (2, V_BOOL false)
+                         ]).
+    Lemma test_valid2 : Valid desc2 val2.
+    Proof.
+      vm_compute.
+      rewrite ?Logic.and_assoc.
+      split; first trivial.
+      split; last (exists false; reflexivity).
+      exists val1. split; first reflexivity.
+      apply test_valid1.
+    Qed.
+
+    Compute Init desc2.
 
   End Desc.
 
+  (** Encoding format *)
+
+  (*
+    Both integer and boolean fields will be encoded into a 4-byte integer so that the descriptor is
+    required to cast them into the correct final form.
+
+    Each primitive field is tagged with the field number as a 1-byte integer, then the 4-byte payload.
+
+    Nested messages still start with a 1-byte field number, and then are followed with a 4-byte length
+    which represents the total encoding length of the nested message.
+
+    Many of the low-level parsers, bytes, integers, bools, etc are taken from SimplParse.v.
+   *)
+
+  Definition to_enc (l : list Z) : list byte := map (fun n => W8 n) l.
+
   Section Parse.
+    Definition ParseByte : P.Parser byte :=
+      fun inp => match inp with
+              | byt :: rest => P.Success byt rest
+              | [] => P.Failure P.Failure.Recoverable (P.Failure.mkData "No more data to parse" inp None)
+              end.
+
+    Definition ParseUnsigned : P.Parser Z := P.Map ParseByte word.unsigned.
+
+    Definition ParseNat : Parser nat := P.Map ParseByte (fun b => Z.to_nat $ word.unsigned b).
+
+    (* Parse n bytes into an unsigned integer *)
+    Definition ParseZN (n : nat) := P.Map (P.RepN ParseUnsigned
+                                         (fun (acc : Z * Z) (new : Z) => let (n, v) := acc in
+                                                                       (n + 8, new ≪ n + v))
+                                         n (0, 0))
+                                    (fun ret => let (_, z) := ret in z).
+
+    Definition ParseZ32 := ParseZN 4%nat.
+
+    Definition ParseBool : Parser bool := P.Map ParseZ32 (fun z => z >? 0).
+
+    Definition ParseVal (parse__msg : Desc -> Parser Value) (d : Desc) : Parser (Z * Val) :=
+      P.Bind ParseUnsigned
+        (fun z =>
+           match (Fields d) !! z with
+           | Some f => match f with
+                      | F_BOOL => P.Map ParseBool (fun b => (z, V_BOOL b))
+                      | F_INT => P.Map ParseZ32 (fun z' => (z, V_INT z'))
+                      | F_MSG d' => P.Map (P.Len ParseNat $ parse__msg d') (fun v => (z, V_MSG v))
+                      end
+           | None => P.SucceedWith (z, V_MISSING)
+           end).
+
+    Definition dummy_msg_parser := fun _ : Desc => P.SucceedWith (VALUE $ gmap_empty).
+
+    Definition fenc1 := to_enc [1; 0; 0; 0; 0].
+    Compute ParseVal dummy_msg_parser desc1 fenc1.
+
+    Definition fenc2 := to_enc [2; 255; 255; 255; 0].
+    Compute ParseVal dummy_msg_parser desc1 fenc2.
+
+    Definition fenc3 := to_enc [1; 8; 0; 0; 0; 0; 0; 0; 0; 0].
+    Compute ParseVal dummy_msg_parser desc2 fenc3.
+
+    Definition Merge (acc : Value) (new : Z * Val) : Value :=
+      let (id, val) := new in
+      (* Only update if the field is already present to drop bad fields *)
+      match (Vals acc) !! id with
+      | Some _ => VALUE $ <[ id := val ]> (Vals acc)
+      | None => acc
+      end.
+
+    Definition ParseValue' (self : Desc -> P.Parser Value) (d : Desc) : Parser Value :=
+      P.Rep (ParseVal self d) Merge (Init d).
+
+    Definition ParseValue (d : Desc) : Parser Value :=
+      P.RecursiveState ParseValue' d.
+
+    Definition enc2 := to_enc [1; 8; 0; 0; 0; 0; 0; 0; 0; 0;
+                               2; 0; 0; 0; 1;
+                               (* Extra field, which is dropped *)
+                               3; 0; 0; 0; 0].
+    Compute ParseValue desc2 enc2.
+
+    Definition desc3 := DESC (list_to_map [
+                                  (1, F_INT);
+                                  (2, F_BOOL);
+                                  (3, F_MSG desc1);
+                                  (4, F_MSG desc2)
+                          ]).
+    Definition val3 := VALUE (list_to_map [
+                                  (1, V_INT 16777215);
+                                  (2, V_BOOL false);
+                                  (3, V_MSG $ VALUE (list_to_map [
+                                                         (1, V_BOOL true);
+                                                         (2, V_INT 3668)
+                                  ]));
+                                  (3, V_MSG $ VALUE (list_to_map [
+                                                         (1, V_MSG val1);
+                                                         (2, V_BOOL true)
+                                  ]))
+                         ]).
+    Definition enc3 := to_enc [
+                           1; 255; 255; 255; 0;
+                           2; 0; 0; 0; 1;
+                           3; 10;
+                                1; 0; 0; 0; 1;
+                                2; 84; 14; 0; 0;
+                           4; 15;
+                                1; 8; 0; 0; 0; 0; 0; 0; 0; 0;
+                                2; 0; 0; 0; 1
+                         ].
+    Definition result3 := fst $ P.Extract (ParseValue desc3 enc3) I.
+    Compute decide (result3 = val3).
   End Parse.
 
   Section Serial.
+    Definition SerialByte : S.Serializer byte S.Trivial_wf :=
+      fun b => S.Success [b].
+
+    Definition SerialUnsigned : S.Serializer Z (fun z => 0 <= z < 256) :=
+      fun z => SerialByte $ W8 z.
+
+    Definition SerialNat : S.Serializer nat (fun n => (0 <= n < 256)%nat) :=
+      fun n => SerialByte $ W8 (Z.of_nat n).
+
+    Definition Z__next (z : Z) : Z :=
+      z ≫ 8.
+
+    (* Create an n-byte little-endian list of z.
+       If z doesn't fit into n bytes, the first n bytes are returned.
+       If z fits into less than n bytes, the list is padded with zeros.
+     *)
+    Fixpoint Z_to_list (z : Z) (n : nat) : list byte :=
+      match n with
+      | O => []
+      | S n' => W8 z :: Z_to_list (Z__next z) n'
+      end.
+
+    Definition SerialZ_wf (n : nat) (z : Z) : Prop :=
+      (0 <= z < 2^(8 * Z.of_nat n)).
+
+    Definition SerialZN (n : nat) : S.Serializer Z (SerialZ_wf n) :=
+      fun z => S.Rep SerialByte (Z_to_list z n).
+
+    Definition SerialZ32 := SerialZN 4%nat.
+
+    Definition SerialBool : S.Serializer bool S.Trivial_wf :=
+      fun b => if b then
+              SerialZ32 1
+            else
+              SerialZ32 0.
+
   End Serial.
 
   Section Theorems.
+    Ltac comp_add := 
+      repeat match goal with
+        | |- context[Z.add ?n ?m] =>
+            match n with Z0 => idtac | Zpos _ => idtac | Zneg _ => idtac end;
+            match m with Z0 => idtac | Zpos _ => idtac | Zneg _ => idtac end;
+            let r := eval compute in (Z.add n m) in 
+              change (Z.add n m) with r
+        end.
+
+    Ltac invc H := inversion H; subst; clear H.
+
+    Theorem ByteParseOk : ParseOk ParseByte SerialByte.
+    Proof.
+      intros x enc rest _.
+      unfold SerialByte.
+      intro H. invc H.
+      reflexivity.
+    Qed.
+
+    Theorem UnsignedParseOk : ParseOk ParseUnsigned SerialUnsigned.
+    Proof.
+      intros x enc rest wf.
+      unfold SerialUnsigned, SerialByte.
+      intros H. invc H.
+      unfold ParseUnsigned, P.Map.
+      simpl. f_equal. word.
+    Qed.
+
+    Theorem NatParseOk : ParseOk ParseNat SerialNat.
+    Proof.
+      intros x enc rest wf.
+      unfold SerialNat, SerialByte.
+      intros H. invc H.
+      unfold ParseNat, P.Map.
+      simpl. f_equal. word.
+    Qed.
+
+    Theorem Z32ParseOk : ParseOk ParseZ32 SerialZ32.
+    Proof.
+    Admitted.
+
+    Theorem BoolParseOk : ParseOk ParseBool SerialBool.
+    Proof.
+      intros x enc rest _.
+      destruct x.
+      - unfold SerialBool. intro H. invc H.
+        vm_compute. reflexivity.
+      - unfold SerialBool. intro H. invc H.
+        vm_compute. reflexivity.
+    Qed.
+
   End Theorems.
 
 End InterParse.
